Remove the TyACap type, specify compose-capability

src/Pact.v
@@ -1,5 +1,6 @@
 Require Export
   Hask.Control.Monad
+  Hask.Control.Lens
   Lib
   Exp
   SemTy
@@ -18,7 +19,10 @@ Section Pact.
 Inductive CapError : Set :=
   | CapErr_CapabilityNotAvailable
   | CapErr_NoResourceAvailable
-  | CapErr_CannotInstallDuringWith.
+  | CapErr_CannotInstallInDefcap
+  | CapErr_CannotWithInDefcap
+  | CapErr_CannotComposeOutsideDefcap
+  | CapErr_CannotWithOutsideDefcapModule.
 
 Derive NoConfusion NoConfusionHom Subterm EqDec for CapError.
 
@@ -30,7 +34,8 @@ Derive NoConfusion NoConfusionHom Subterm EqDec for Err.
 
 Inductive EvalContext : Set :=
   | RegularEvaluation
-  | InWithCapability.
+  | InWithCapability
+  | InModule : string → EvalContext.
 
 Derive NoConfusion NoConfusionHom Subterm EqDec for EvalContext.
 
@@ -38,22 +43,47 @@ Record PactEnv : Set := {
   (* We cannot refer to capability tokens by their type here, because
      capability predicates execute in a state monad that reference this
      record type. *)
-  granted : list ACap;
-  context : list EvalContext;
+  _granted : list ACap;
+  _context : list EvalContext;
 }.
 
 Derive NoConfusion NoConfusionHom Subterm EqDec for PactEnv.
+
+Definition granted : Lens' PactEnv (list ACap) :=
+  λ _ _ f env,
+    f (_granted env) <&> λ g,
+      {| _granted := g
+       ; _context := _context env |}.
+
+Definition context : Lens' PactEnv (list EvalContext) :=
+  λ _ _ f env,
+    f (_context env) <&> λ c,
+      {| _granted := _granted env
+       ; _context := c |}.
 
 Record PactState : Set := {
   (* We cannot refer to capability tokens by their type here, because
      capability predicates execute in a state monad that reference this
      record type. *)
-  resources : list ACap;
+  _resources  : list ACap;
+  _to_compose : list ACap;
 }.
 
 Derive NoConfusion NoConfusionHom Subterm EqDec for PactState.
 
-Record PactLog : Set := {}.
+Definition resources : Lens' PactState (list ACap) :=
+  λ _ _ f env,
+    f (_resources env) <&> λ r,
+      {| _resources  := r
+       ; _to_compose := _to_compose env |}.
+
+Definition to_compose : Lens' PactState (list ACap) :=
+  λ _ _ f env,
+    f (_to_compose env) <&> λ tc,
+      {| _resources  := _resources env
+       ; _to_compose := tc |}.
+
+Record PactLog : Set := MkLog {}.
 
 Derive NoConfusion NoConfusionHom Subterm EqDec for PactLog.
 
@@ -62,5 +92,44 @@ Definition PactM : Type → Type := @RWSE PactEnv PactState PactLog Err.
 #[export] Instance PactM_Functor     : Functor PactM     := RWSE_Functor.
 #[export] Instance PactM_Applicative : Applicative PactM := RWSE_Applicative.
 #[export] Instance PactM_Monad       : Monad PactM       := RWSE_Monad.
+
+Definition uncurryM `(f : a → PactM (b → PactM c)) : (a * b) → PactM c :=
+  λ '(a, b), f' <- f a ; f' b.
+
+(* This is not a valid definition. *)
+Definition curryM `(f : (a * b) → PactM c) : a → PactM (b → PactM c) :=
+  pure ∘ curry f.
+
+Lemma uncurryM_curryM `(f : (a * b) → PactM c) :
+  uncurryM (curryM f) = f.
+Proof.
+  extensionality p.
+  destruct p.
+  unfold uncurryM, curryM.
+  simpl.
+  unfold RWSE_join.
+  extensionality r.
+  extensionality s.
+  extensionality w.
+  f_equal.
+  destruct w.
+  reflexivity.
+Qed.
+
+Lemma curryM_uncurryM `(f : a → PactM (b → PactM c)) :
+  curryM (uncurryM f) = f.
+Proof.
+  extensionality x.
+  unfold uncurryM, curryM.
+  simpl.
+  unfold RWSE_join.
+  extensionality r.
+  extensionality s.
+  extensionality w.
+  unfold Basics.compose.
+  unfold curry.
+  unfold Tuple.first.
+  unfold Either.Either_map.
+Abort.
 
 End Pact.
