src/Exp.v
@@ -81,15 +81,16 @@ Inductive Exp Γ : Ty → Set :=
   | WithCapability {p v τ} :
     ConcreteP p →
     ConcreteP v →
-    Exp Γ (TyCap p v ⟶ TyList TyACap) →
-    Exp Γ (v × v ⟶ v) →
+    Exp Γ TySym →                (* name of the defining module *)
+    Exp Γ (TyCap p v ⟶ 𝕌) →     (* throws exception on failure *)
+    Exp Γ (v × v ⟶ v) →         (* throws exception on failure *)
     Exp Γ (TyCap p v) → Exp Γ τ → Exp Γ τ
 
   | ComposeCapability {p v} :
     ConcreteP p →
     ConcreteP v →
-    Exp Γ (TyCap p v ⟶ TyList TyACap) →
-    Exp Γ (v × v ⟶ v) →
+    Exp Γ (TyCap p v ⟶ 𝕌) →     (* throws exception on failure *)
+    Exp Γ (v × v ⟶ v) →         (* throws exception on failure *)
     Exp Γ (TyCap p v) → Exp Γ 𝕌
 
   | InstallCapability {p v} : Exp Γ (TyCap p v) → Exp Γ 𝕌
@@ -119,8 +120,8 @@ Fixpoint Exp_size {Γ τ} (e : Exp Γ τ) : nat :=
   | Seq _ x y   => 1 + Exp_size x + Exp_size y
 
   | Capability _ _ _ n p v => 1 + Exp_size n + Exp_size p + Exp_size v
-  | WithCapability _ _ _ p m c e =>
-      1 + Exp_size p + Exp_size m + Exp_size c + Exp_size e
+  | WithCapability _ _ _ nm p m c e =>
+      1 + Exp_size nm + Exp_size p + Exp_size m + Exp_size c + Exp_size e
   | ComposeCapability _ _ _ p m c =>
       1 + Exp_size p + Exp_size m + Exp_size c
   | InstallCapability _ c => 1 + Exp_size c
@@ -154,7 +155,7 @@ Arguments Cdr {Γ τ} _.
 Arguments IsNil {Γ τ} _.
 Arguments Seq {Γ τ τ'} _ _.
 Arguments Capability {_ p v} _ _ _.
-Arguments WithCapability {_ p v τ} _ _ _ _ _ _.
+Arguments WithCapability {_ p v τ} _ _ _ _ _ _ _.
 Arguments ComposeCapability {_ p v} _ _ _ _ _.
 Arguments InstallCapability {_ p v} _.
 Arguments RequireCapability {_ p v} _.
