src/Ty.v
@@ -28,7 +28,6 @@ Inductive Ty : Set :=
   | TyList  : Ty → Ty
   | TyPair  : Ty → Ty → Ty
 
-  | TyACap  : Ty
   | TyCap   : Ty → Ty → Ty.
 
 Derive NoConfusion NoConfusionHom Subterm EqDec for Ty.
